theories/Pipeline.v
@@ -7,7 +7,7 @@
 From MetaRocq.Template Require Import All.
 From MetaRocq.Utils Require Import bytestring MRString.
 From MetaRocq.Common Require Import Kernames Environment.
-From Hallmark Require Import Lookup Translate Emit Clause.
+From Hallmark Require Import Lookup Translate Emit Clause Clp.
 From Stdlib Require Import List.
 Import ListNotations.
 
@@ -49,16 +49,17 @@ Definition build_env (decls : global_declarations) : global_env :=
      declarations := decls;
      retroknowledge := Retroknowledge.empty |}.
 
-Definition translate_all (Σ : global_env) (inds : list inductive)
-  : list clause :=
+Definition translate_all (tbl : clp_table) (Σ : global_env)
+  (inds : list inductive) : list clause :=
   flat_map (fun ind =>
     match find_inductive Σ (inductive_mind ind) with
-    | Some mib => translate_inductive Σ ind mib
+    | Some mib => translate_inductive tbl Σ ind mib
     | None => []
     end) inds.
 
 (** Translate every inductive in a module to a Prolog program. *)
 Definition hallmark_module (mod_name : qualid) : TemplateMonad string :=
+  tmBind clpfd_defaults (fun tbl =>
   tmBind (tmQuoteModule mod_name) (fun refs =>
     let inds := filter_ind_refs refs in
     match inds with
@@ -67,6 +68,6 @@ Definition hallmark_module (mod_name : qualid) : TemplateMonad string :=
       let kns := collect_kernames inds in
       tmBind (quote_all kns) (fun decls =>
         let Σ := build_env decls in
-        let all_clauses := translate_all Σ inds in
+        let all_clauses := translate_all tbl Σ inds in
         tmReturn (print_program all_clauses))
-    end).
+    end)).
