theories/Translate.v
@@ -11,25 +11,55 @@
 
 From MetaRocq.Template Require Import All.
 From MetaRocq.Utils Require Import bytestring MRString.
-From Hallmark Require Import Clause Telescope Classify Lookup.
+From Hallmark Require Import Clause Telescope Classify Lookup Clp.
 From Stdlib Require Import List.
 Import ListNotations.
 
+(** Check whether a kername refers to [nat] by its short name. *)
+Definition is_nat_kn (kn : kername) : bool :=
+  String.eqb (snd kn) "nat"%bs.
+
+(** Try to read a Peano nat literal from the MetaRocq AST.
+    [O] is [tConstruct nat 0], [S n] is [tApp (tConstruct nat 1) [n]].
+    Only matches constructors of the [nat] inductive. *)
+Fixpoint read_nat (fuel : nat) (t : term) : option nat :=
+  match fuel with
+  | 0 => None
+  | S fuel' =>
+    match t with
+    | tConstruct (mkInd kn 0) 0 _ =>
+      if is_nat_kn kn then Some 0 else None
+    | tApp (tConstruct (mkInd kn 0) 1 _) [x] =>
+      if is_nat_kn kn then
+        match read_nat fuel' x with
+        | Some n => Some (S n)
+        | None   => None
+        end
+      else None
+    | _ => None
+    end
+  end.
+
 (** Map a MetaRocq [term] to a [prolog_term].
     [depth] is the number of enclosing binders; [tRel n] is
-    normalized to canonical binding position [depth - 1 - n]. *)
+    normalized to canonical binding position [depth - 1 - n].
+    Peano nat literals are converted to integer atoms. *)
 Definition term_to_prolog (Σ : global_env) (depth : nat) (t : term)
   : prolog_term :=
-  match t with
-  | tRel n => PVar (depth - 1 - n)
-  | tConstruct ind idx _ =>
-    match lookup_constructor_name Σ ind idx with
-    | Some name => PAtom name
-    | None => PAtom "?"%bs
+  match read_nat 1000 t with
+  | Some n => PAtom (string_of_nat n)
+  | None =>
+    match t with
+    | tRel n => PVar (depth - 1 - n)
+    | tConstruct ind idx _ =>
+      match lookup_constructor_name Σ ind idx with
+      | Some name => PAtom name
+      | None => PAtom "?"%bs
+      end
+    | tConst kn _ => PAtom (snd kn)
+    | tInd (mkInd kn _) _ => PAtom (snd kn)
+    | _ => PAtom "?"%bs
     end
-  | tConst kn _ => PAtom (snd kn)
-  | tInd (mkInd kn _) _ => PAtom (snd kn)
-  | _ => PAtom "?"%bs
   end.
 
 Definition args_to_prolog (Σ : global_env) (depth : nat) (args : list term)
@@ -46,7 +76,8 @@ Definition extract_conclusion (Σ : global_env) (ind_kn : kername)
   end.
 
 (** Collect clause body atoms from classified bindings.
-    Each binding at index [i] has its args at depth [i]. *)
+    Each binding at index [i] has its args at depth [i].
+    [BConstraint] bindings become [PConstraint op lhs rhs]. *)
 Definition extract_body (Σ : global_env) (ind_kn : kername)
   (classes : list binding_class) : list prolog_term :=
   let fix go (i : nat) (cs : list binding_class) : list prolog_term :=
@@ -56,6 +87,14 @@ Definition extract_body (Σ : global_env) (ind_kn : kername)
       (match bc with
        | BRecursive args => [PApp (snd ind_kn) (args_to_prolog Σ i args)]
        | BExternal head args => [PApp (snd head) (args_to_prolog Σ i args)]
+       | BConstraint op args =>
+         match args with
+         | [a1; a2] =>
+           [PConstraint op (term_to_prolog Σ i a1) (term_to_prolog Σ i a2)]
+         | [_; a1; a2] =>
+           [PConstraint op (term_to_prolog Σ i a1) (term_to_prolog Σ i a2)]
+         | _ => []
+         end
        | BIndex | BErased => []
        end) ++ go (S i) rest
     end
@@ -75,6 +114,8 @@ Fixpoint build_witness_args_aux (cs : list binding_class) (i body_idx : nat)
     | BRecursive _ | BExternal _ _ =>
       PApp "pf"%bs [PAtom (string_of_nat body_idx)]
         :: build_witness_args_aux rest (S i) (S body_idx)
+    | BConstraint _ _ =>
+      PAtom "lia"%bs :: build_witness_args_aux rest (S i) (S body_idx)
     | BErased => build_witness_args_aux rest (S i) body_idx
     end
   end.
@@ -86,11 +127,11 @@ Definition build_witness_args (classes : list binding_class) : list prolog_term 
     For nullary constructors (empty telescope, no conclusion args),
     the constructor name is injected as an atom argument in the head:
     e.g. [admin : user] becomes [user(admin).] *)
-Definition translate_constructor (Σ : global_env) (ind_kn : kername)
-  (name : ident) (ty : term) : option clause :=
+Definition translate_constructor (tbl : clp_table) (Σ : global_env)
+  (ind_kn : kername) (name : ident) (ty : term) : option clause :=
   let '(bindings, ret) := parse_telescope ty in
   let total := length bindings in
-  let classes := classify_all ind_kn bindings in
+  let classes := classify_all tbl ind_kn bindings in
   match extract_conclusion Σ ind_kn total ret with
   | Some head =>
     let head' :=
@@ -113,14 +154,14 @@ Definition instantiate_cstr (mib : mutual_inductive_body) (ind : inductive)
   remove_arity (ind_npars mib) (subst0 subs (cstr_type cdecl)).
 
 (** Translate every constructor of an inductive into Prolog clauses. *)
-Definition translate_inductive (Σ : global_env) (ind : inductive)
-  (mib : mutual_inductive_body) : list clause :=
+Definition translate_inductive (tbl : clp_table) (Σ : global_env)
+  (ind : inductive) (mib : mutual_inductive_body) : list clause :=
   let ind_kn := inductive_mind ind in
   match nth_error (ind_bodies mib) (inductive_ind ind) with
   | Some oib =>
     flat_map (fun cdecl =>
       let ty := instantiate_cstr mib ind cdecl in
-      match translate_constructor Σ ind_kn (cstr_name cdecl) ty with
+      match translate_constructor tbl Σ ind_kn (cstr_name cdecl) ty with
       | Some c => [c]
       | None => []
       end
